src/coq/Handlers/Handlers.v
@@ -32,51 +32,12 @@ From Vellvm.Handlers Require Export
 From Vellvm.Semantics Require Import Memory.Sizeof Memory.MemBytes GepM.
 
 (* Handlers get instantiated over the domain of addresses provided by the memory model *)
-Module LLVMEvents64 := LLVMEvents.Make(MemoryModelImplementation.Addr)(MemoryModelImplementation.IP64Bit)(MemoryModelImplementation.FinSizeof).
-Module Global64 := Global.Make MemoryModelImplementation.Addr MemoryModelImplementation.IP64Bit MemoryModelImplementation.FinSizeof LLVMEvents64.
-Module Local64  := Local.Make  MemoryModelImplementation.Addr MemoryModelImplementation.IP64Bit MemoryModelImplementation.FinSizeof LLVMEvents64.
-Module Stack64  := Stack.Make  MemoryModelImplementation.Addr MemoryModelImplementation.IP64Bit MemoryModelImplementation.FinSizeof LLVMEvents64.
+Module LLVMEvents64 := LLVMEvents.Make(MemoryModelImplementation.FinAddr)(MemoryModelImplementation.IP64Bit)(MemoryModelImplementation.FinSizeof).
+Module Global64 := Global.Make MemoryModelImplementation.FinAddr MemoryModelImplementation.IP64Bit MemoryModelImplementation.FinSizeof LLVMEvents64.
+Module Local64  := Local.Make  MemoryModelImplementation.FinAddr MemoryModelImplementation.IP64Bit MemoryModelImplementation.FinSizeof LLVMEvents64.
+Module Stack64  := Stack.Make  MemoryModelImplementation.FinAddr MemoryModelImplementation.IP64Bit MemoryModelImplementation.FinSizeof LLVMEvents64.
 
-Module LLVMEvents := LLVMEvents.Make(MemoryModelImplementation.Addr)(MemoryModelImplementation.BigIP)(MemoryModelImplementation.FinSizeof).
-Module Global := Global.Make MemoryModelImplementation.Addr MemoryModelImplementation.BigIP MemoryModelImplementation.FinSizeof LLVMEvents.
-Module Local  := Local.Make  MemoryModelImplementation.Addr MemoryModelImplementation.BigIP MemoryModelImplementation.FinSizeof LLVMEvents.
-Module Stack  := Stack.Make  MemoryModelImplementation.Addr MemoryModelImplementation.BigIP MemoryModelImplementation.FinSizeof LLVMEvents.
-
-Require Import List.
-
-Import ListNotations.
-
-From Vellvm Require Import
-     Utils.Error
-     Semantics.MemoryAddress
-     Semantics.LLVMEvents
-     DynamicTypes.
-
-From ExtLib Require Import
-     Structures.Monad.
-
-Import MonadNotation.
-
-(* Module GEP := GepM.Make MemoryModelImplementation.Addr MemoryModelImplementation.BigIP MemoryModelImplementation.FinSizeof LLVMEvents MemoryModelImplementation.FinPTOI MemoryModelImplementation.FinPROV MemoryModelImplementation.FinITOP. *)
-(* Module GEP64 := GepM.Make MemoryModelImplementation.Addr MemoryModelImplementation.IP64Bit MemoryModelImplementation.FinSizeof LLVMEvents64 MemoryModelImplementation.FinPTOI MemoryModelImplementation.FinPROV MemoryModelImplementation.FinITOP. *)
-
-(* Module Intrinsics64 := Intrinsics.Make MemoryModelImplementation.Addr MemoryModelImplementation.IP64Bit MemoryModelImplementation.FinSizeof LLVMEvents64. *)
-(* Module Intrinsics := Intrinsics.Make MemoryModelImplementation.Addr MemoryModelImplementation.BigIP MemoryModelImplementation.FinSizeof LLVMEvents. *)
-
-(* Module Byte := FinByte MemoryModelImplementation.Addr MemoryModelImplementation.BigIP MemoryModelImplementation.FinSizeof LLVMEvents. *)
-(* Module Byte64 := FinByte MemoryModelImplementation.Addr MemoryModelImplementation.IP64Bit MemoryModelImplementation.FinSizeof LLVMEvents64. *)
-
-(* Module SER := Serialization.Make(MemoryModelImplementation.Addr)(MemoryModelImplementation.BigIP)(MemoryModelImplementation.FinSizeof)(LLVMEvents)(MemoryModelImplementation.FinPTOI)(MemoryModelImplementation.FinPROV)(MemoryModelImplementation.FinITOP)(GEP)(Byte). *)
-(* Module SER64 := Serialization.Make(MemoryModelImplementation.Addr)(MemoryModelImplementation.IP64Bit)(MemoryModelImplementation.FinSizeof)(LLVMEvents64)(MemoryModelImplementation.FinPTOI)(MemoryModelImplementation.FinPROV)(MemoryModelImplementation.FinITOP)(GEP64)(Byte64). *)
-
-(* Module MEM := MemoryModelImplementation.Make(MemoryModelImplementation.Addr)(MemoryModelImplementation.BigIP)(MemoryModelImplementation.FinSizeof)(LLVMEvents)(MemoryModelImplementation.FinPTOI)(MemoryModelImplementation.FinPROV)(MemoryModelImplementation.FinITOP)(GEP)(Byte). *)
-(* Module MEM64 := MemoryModelImplementation.Make(MemoryModelImplementation.Addr)(MemoryModelImplementation.IP64Bit)(MemoryModelImplementation.FinSizeof)(LLVMEvents64)(MemoryModelImplementation.FinPTOI)(MemoryModelImplementation.FinPROV)(MemoryModelImplementation.FinITOP)(GEP64)(Byte64). *)
-
-(* Module MEMORY_THEORY := MemoryModelImplementationTheory.Make(MemoryModelImplementation.Addr)(MemoryModelImplementation.BigIP)(MemoryModelImplementation.FinSizeof)(LLVMEvents)(MemoryModelImplementation.FinPTOI)(MemoryModelImplementation.FinPROV)(MemoryModelImplementation.FinITOP)(GEP)(Byte). *)
-(* Module MEMORY_THEORY64 := MemoryModelImplementationTheory.Make(MemoryModelImplementation.Addr)(MemoryModelImplementation.IP64Bit)(MemoryModelImplementation.FinSizeof)(LLVMEvents64)(MemoryModelImplementation.FinPTOI)(MemoryModelImplementation.FinPROV)(MemoryModelImplementation.FinITOP)(GEP64)(Byte64). *)
-
-(* Module Pick64 := Pick.Make MemoryModelImplementation.Addr MemoryModelImplementation.IP64Bit FinSizeof LLVMEvents64 FinPTOI FinPROV FinITOP GEP64 Byte64. *)
-(* Module Pick := Pick.Make MemoryModelImplementation.Addr MemoryModelImplementation.BigIP FinSizeof LLVMEvents FinPTOI FinPROV FinITOP GEP Byte. *)
-
-(* Export LLVMEvents LLVMEvents.DV Global Local Stack Pick Intrinsics *)
-(*        MEM MEMORY_THEORY UndefinedBehaviour. *)
+Module LLVMEvents := LLVMEvents.Make(MemoryModelImplementation.InfAddr)(MemoryModelImplementation.BigIP)(MemoryModelImplementation.FinSizeof).
+Module Global := Global.Make MemoryModelImplementation.InfAddr MemoryModelImplementation.BigIP MemoryModelImplementation.FinSizeof LLVMEvents.
+Module Local  := Local.Make  MemoryModelImplementation.InfAddr MemoryModelImplementation.BigIP MemoryModelImplementation.FinSizeof LLVMEvents.
+Module Stack  := Stack.Make  MemoryModelImplementation.InfAddr MemoryModelImplementation.BigIP MemoryModelImplementation.FinSizeof LLVMEvents.
