src/coq/Handlers/MemoryModel.v
@@ -234,6 +234,7 @@ Module MemoryHelpers (LP : LLVMParams) (MP : MemoryParams LP) (Byte : ByteModule
   Import LP.Events.
   Import LP.SIZEOF.
   Import LP.PTOI.
+  Import LP.ITOP.
   Import LP.PROV.
   Import IP.
   Import Byte.
@@ -608,10 +609,11 @@ Module MemoryHelpers (LP : LLVMParams) (MP : MemoryParams LP) (Byte : ByteModule
 
   Definition get_consecutive_ptrs {M} `{Monad M} `{RAISE_OOM M} `{RAISE_ERROR M} (ptr : addr) (len : nat) : M (list addr) :=
     ixs <- lift_OOM (intptr_seq 0 len);;
-    lift_err_RAISE_ERROR
-      (map_monad
-         (fun ix => handle_gep_addr (DTYPE_I 8) ptr [DVALUE_IPTR ix])
-         ixs).
+    addrs <- lift_err_RAISE_ERROR
+              (map_monad
+                 (fun ix => handle_gep_addr (DTYPE_I 8) ptr [DVALUE_IPTR ix])
+                 ixs (m:=err));;
+    lift_OOM (sequence addrs).
 
   Ltac convert_to_ret :=
     match goal with
@@ -693,17 +695,28 @@ Module MemoryHelpers (LP : LLVMParams) (MP : MemoryParams LP) (Byte : ByteModule
         (* TODO: need inversion lemma. *)
         cbn in CONSEC.
         convert_to_ret_hyp.
-          eapply rw_ret_nin_raise in CONSEC; [contradiction | auto].
+        setoid_rewrite rbm_raise_bind in CONSEC; auto.
+        eapply rw_ret_nin_raise in CONSEC; [contradiction | auto].
       + cbn in CONSEC.
         convert_to_ret_hyp.
-        apply within_ret_ret in CONSEC; auto.
-        assert (MReturns l0 (map_monad (fun ix : IP.intptr => handle_gep_addr (DTYPE_I 8) ptr [DVALUE_IPTR ix]) l)) as RETS.
-        { auto. }
+        setoid_rewrite bind_ret_l in CONSEC.
+        destruct (sequence l0) eqn:HSEQUENCE.
+        { cbn in CONSEC.
+          apply within_ret_ret in CONSEC; auto.
+          assert (MReturns l0 (map_monad (fun ix : IP.intptr => handle_gep_addr (DTYPE_I 8) ptr [DVALUE_IPTR ix]) l)) as RETS.
+          { auto. }
 
-        epose proof MapMonadExtra.map_monad_length l _ _ RETS as LEN.
-        apply intptr_seq_len in SEQ.
-        subst.
-        auto.
+          epose proof MapMonadExtra.map_monad_length l _ _ RETS as LEN.
+          apply intptr_seq_len in SEQ.
+          subst.
+          auto.
+
+          apply sequence_OOM_length in HSEQUENCE.
+          lia.
+        }
+        { cbn in *.
+          eapply rw_ret_nin_raise in CONSEC; [contradiction | auto].
+        }
     - (* OOM: CONSEC equivalent to ret is a contradiction. *)
       cbn in CONSEC.
       setoid_rewrite rbm_raise_bind in CONSEC; auto.
@@ -745,22 +758,24 @@ Module MemoryHelpers (LP : LLVMParams) (MP : MemoryParams LP) (Byte : ByteModule
                      MP.GEP.handle_gep_addr (DTYPE_I 8) ptr [Events.DV.DVALUE_IPTR ix])
                   l) eqn:HMAPM.
       + cbn in CONSEC.
-        convert_to_ret_hyp;
-          eapply rw_ret_nin_raise in CONSEC; [contradiction | try typeclasses eauto].
+        setoid_rewrite rbm_raise_bind in CONSEC; auto.
+        eapply rw_ret_nin_raise in CONSEC; [contradiction | try typeclasses eauto].
       + cbn in CONSEC.
-        convert_to_ret_hyp.
-        apply within_ret_ret in CONSEC; eauto.
-        inv CONSEC.
+        setoid_rewrite bind_ret_l in CONSEC.
+        rename l0 into addrs.
+        destruct (sequence addrs) eqn:HSEQUENCE.
+        { apply within_ret_ret in CONSEC; eauto.
+          inv CONSEC.
 
-        pose proof (@exists_in_bounds_le_lt
-                      (ptr_to_int ptr)
-                      (ptr_to_int ptr + Z.of_nat len)
-                      ix) as BOUNDS.
+          pose proof (@exists_in_bounds_le_lt
+                        (ptr_to_int ptr)
+                        (ptr_to_int ptr + Z.of_nat len)
+                        ix) as BOUNDS.
 
-        forward BOUNDS. lia.
-        destruct BOUNDS as [offset [[BOUNDLE BOUNDLT] EQ]].
+          forward BOUNDS. lia.
+          destruct BOUNDS as [offset [[BOUNDLE BOUNDLT] EQ]].
 
-        (* How does ix connect to HSEQ?
+          (* How does ix connect to HSEQ?
 
                        EQ: ix = ptr_to_int ptr + offset
                        BOUNDLE : 0 <= offset
@@ -775,27 +790,82 @@ Module MemoryHelpers (LP : LLVMParams) (MP : MemoryParams LP) (Byte : ByteModule
                        exists ip_offset, In ip_offset l /\ from_Z ip_offset = offset
 
                        (or maybe to_Z ip_offset = NoOom offset)
-         *)
-        pose proof intptr_seq_from_Z 0 len l HSEQ offset as FROMZ.
-        forward FROMZ; [lia|].
-        destruct FROMZ as (ip_offset & FROMZ & INSEQ).
+           *)
+          pose proof intptr_seq_from_Z 0 len l HSEQ offset as FROMZ.
+          forward FROMZ; [lia|].
+          destruct FROMZ as (ip_offset & FROMZ & INSEQ).
 
-        eapply (@map_monad_err_In' err _ _ Monads.MonadLaws_sum) with (y:=ip_offset) in HMAPM; auto; try typeclasses eauto.
+          eapply (@map_monad_err_In' err _ _ Monads.MonadLaws_sum) with (y:=ip_offset) in HMAPM; auto; try typeclasses eauto.
 
-        destruct HMAPM as (p' & GEP & IN).
-        symmetry in GEP.
-        cbn in GEP.
-        apply MP.GEP.handle_gep_addr_ix in GEP.
-        exists p'. split; auto.
-        subst.
+          destruct HMAPM as (p' & GEP & IN).
+          symmetry in GEP.
+          cbn in GEP.
+          destruct p' as [p' | oom_msg].
+          { apply MP.GEP.handle_gep_addr_ix in GEP.
+            exists p'. split; auto.
+            subst.
 
-        rewrite sizeof_dtyp_i8 in GEP.
-        erewrite IP.from_Z_to_Z in GEP; [|apply FROMZ].
-        lia.
+            rewrite sizeof_dtyp_i8 in GEP.
+            erewrite IP.from_Z_to_Z in GEP; [|apply FROMZ].
+            lia.
+
+            unfold sequence in HSEQUENCE.
+
+            (* TODO: move *)
+            Set Nested Proofs Allowed.
+            Lemma sequence_OOM_In :
+              forall {A} (ms : list (OOM A)) xs x,
+                sequence ms = NoOom xs ->
+                In (NoOom x) ms ->
+                In x xs.
+            Proof.
+              intros A.
+              induction ms; intros xs x SEQUENCE IN.
+              - inversion IN.
+              - inversion IN; subst.
+                + cbn in *.
+                  destruct (map_monad id ms) eqn:MAP; inversion SEQUENCE; subst.
+                  cbn; auto.
+                + cbn in *.
+                  destruct a; cbn in *; [|inversion SEQUENCE].
+                  destruct (map_monad id ms) eqn:MAP; inversion SEQUENCE; subst.
+                  right.
+                  eauto.
+            Qed.
+                
+            eapply sequence_OOM_In; eauto.
+          }
+          { subst.
+
+            (* TODO: move *)
+            Lemma sequence_OOM_NoOom_In :
+              forall {A} (ms : list (OOM A)) (xs : list A),
+                sequence ms = NoOom xs ->
+                forall (oom_msg : string), ~ In (Oom oom_msg) ms.
+            Proof.
+              intros A.
+              induction ms; intros xs SEQUENCE msg IN.
+              - inversion IN.
+              - inversion IN; subst.
+                + cbn in *.
+                  inversion SEQUENCE.
+                + cbn in *.
+                  destruct a; inversion SEQUENCE.
+                  destruct (map_monad id ms) eqn:MAP; inversion SEQUENCE; subst.
+                  eapply IHms in H; eauto.
+            Qed.
+
+            eapply sequence_OOM_NoOom_In in HSEQUENCE.
+            apply HSEQUENCE in IN.
+            contradiction.    
+          }
+        }
+        { cbn in *.
+          eapply rw_ret_nin_raise in CONSEC; [contradiction | typeclasses eauto].
+        }
     - cbn in CONSEC.
       setoid_rewrite rbm_raise_bind in CONSEC; [|typeclasses eauto].
-      convert_to_ret_hyp;
-        eapply rw_ret_nin_raise in CONSEC; [contradiction | typeclasses eauto].
+      eapply rw_ret_nin_raise in CONSEC; [contradiction | typeclasses eauto].
   Qed.
 
   Lemma get_consecutive_ptrs_covers_range_eq1 :
@@ -865,7 +935,7 @@ Module MemoryHelpers (LP : LLVMParams) (MP : MemoryParams LP) (Byte : ByteModule
     - cbn in SEQ.
       inv SEQ.
       cbn in CONSEC.
-      convert_to_ret_hyp.
+      setoid_rewrite bind_ret_l in CONSEC.
       eapply within_ret_ret in CONSEC; [|typeclasses eauto].
       inv CONSEC.
     - rewrite intptr_seq_succ in SEQ.
@@ -884,7 +954,7 @@ Module MemoryHelpers (LP : LLVMParams) (MP : MemoryParams LP) (Byte : ByteModule
       break_match_hyp.
       { (* map_monad fails *)
         cbn in CONSEC.
-        convert_to_ret_hyp.
+        setoid_rewrite rbm_raise_bind in CONSEC; eauto.
         apply rw_ret_nin_raise in CONSEC; eauto.
         contradiction.
       }
@@ -892,44 +962,49 @@ Module MemoryHelpers (LP : LLVMParams) (MP : MemoryParams LP) (Byte : ByteModule
       (* map_monad succeeds *)
       cbn in CONSEC.
       convert_to_ret_hyp.
-      eapply within_ret_ret in CONSEC; eauto.
-      inv CONSEC.
-      split; auto.
-
-      destruct len.
-      + cbn in Heqo0.
-        inv Heqo0.
-        cbn in Heqs.
-        inv Heqs.
-        exists ptr. exists 0%nat.
-        split; auto.
-        cbn.
-        setoid_rewrite bind_ret_l.
-        cbn.
-        eapply within_ret_refl; eauto.
-      + pose proof Heqo0 as SEQ.
-        rewrite intptr_seq_succ in SEQ.
-        cbn in SEQ.
-        break_match_hyp; [| solve [inv SEQ]].
-        rename i into one.
-
-        break_match_hyp; [| solve [inv SEQ]].
-        inv SEQ.
-
-        pose proof Heqs as MAPM.
-        rewrite map_monad_unfold in MAPM.
-        cbn in MAPM.
-        break_match_hyp; [ solve [inv MAPM] |].
-        break_match_hyp; [ solve [inv MAPM] |].
-        rename a into p'.
-        rename l1 into ptrs'.
-        inv MAPM.
-
-        exists p'.
-        exists (S len).
+      setoid_rewrite bind_ret_l in CONSEC.
+      destruct (sequence (NoOom ptr :: l)) eqn:SEQUENCE.
+      { eapply within_ret_ret in CONSEC; eauto.
+        inv CONSEC.
+        inv SEQUENCE.
+        break_match_hyp; inv H0.
         split; auto.
 
-      (* Need something about sequences *)
+        destruct len.
+        + cbn in Heqo0.
+          inv Heqo0.
+          cbn in Heqs.
+          inv Heqs.
+          inv Heqo.
+          exists p. exists 0.
+          split; auto.
+          cbn.
+          setoid_rewrite bind_ret_l.
+          cbn.
+          setoid_rewrite bind_ret_l.
+          cbn.
+          apply within_ret_refl; typeclasses eauto.
+        + pose proof Heqo0 as SEQ.
+          rewrite intptr_seq_succ in SEQ.
+          cbn in SEQ.
+          break_match_hyp; [| solve [inv SEQ]].
+          rename i into one.
+
+          break_match_hyp; [| solve [inv SEQ]].
+          inv SEQ.
+
+          pose proof Heqs as MAPM.
+          rewrite map_monad_unfold in MAPM.
+          cbn in MAPM.
+          break_match_hyp; [ solve [inv MAPM] |].
+          break_match_hyp; [ solve [inv MAPM] |].
+          inv MAPM.
+          destruct o as [p' | oom_msg]; [|inversion Heqo].
+          rename l1 into ptrs'.
+          exists p'. exists (S len).
+          split; auto.
+
+          (* Need something about sequences *)
       (* Since len is the length, `intptr_seq 1 len` is basically just `map (+1) (intptr_seq 0 len)` *)
       (* Unfortunately, I don't think I have a lemma that gives me
          `IP.from_Z (x+1) = NoOom (i+1) -> IP.from_Z (x+1) = NoOom i`
@@ -947,16 +1022,16 @@ Module MemoryHelpers (LP : LLVMParams) (MP : MemoryParams LP) (Byte : ByteModule
        *)
 
         rename l0 into ixs.
-        pose proof Heqo0 as SEQ.
+        pose proof Heqo0 as SEQ_SHIFT.
         apply intptr_seq_shifted in Heqo0.
-        destruct Heqo0 as [l'' [SEQ_SHIFT SHIFT]].
-        rewrite SEQ_SHIFT.
+        destruct Heqo0 as [ixs_unshifted [SEQ SHIFT]].
+        rewrite SEQ.
         cbn.
 
         setoid_rewrite bind_ret_l.
         match goal with
         | _ : _ |- context [map_monad ?f ?l] =>
-            assert (map_monad f l = inr (p' :: ptrs')) as Heqs'
+            assert (map_monad f l = inr (NoOom p' :: ptrs')) as Heqs'
         end.
         {
           eapply map_monad_eqv; eauto.
@@ -967,48 +1042,163 @@ Module MemoryHelpers (LP : LLVMParams) (MP : MemoryParams LP) (Byte : ByteModule
           }
 
           intros n a b NTH NTH'.
-          pose proof (intptr_seq_nth _ _ _ _ _ SEQ NTH) as IX.
-          pose proof (intptr_seq_nth _ _ _ _ _ SEQ_SHIFT NTH') as IX'.
+          pose proof (intptr_seq_nth _ _ _ _ _ SEQ_SHIFT NTH) as IX.
+          pose proof (intptr_seq_nth _ _ _ _ _ SEQ NTH') as IX'.
           cbn in IX'.
 
-          apply handle_gep_addr_ix in Heqs0.
-          erewrite handle_gep_addr_ix'.
-          erewrite handle_gep_addr_ix'.
-          reflexivity.
-          reflexivity.
+          (* TODO: move *)
+          (* TODO: can I generalize this? *)
+          Lemma map_monad_OOM_Nth :
+            forall {A B} (f : A -> OOM B) l res x n,
+              map_monad f l = ret res ->
+              Util.Nth res n x ->
+              exists y, f y = ret x /\ Util.Nth l n y.
+          Proof.
+            intros A B f l res x n MAP NTH.
+            generalize dependent l. generalize dependent n. revert x.
+            induction res; intros x n NTH l MAP.
+            - inversion NTH.
+              rewrite nth_error_nil in *; inv H0.
+            - cbn in NTH.
+              induction n.
+              + cbn in NTH.
+                inv NTH.
 
-          assert (address_provenance p' = address_provenance ptr) as PROV.
-          { rewrite map_monad_unfold in Heqs.
-            cbn in Heqs.
-            break_match_hyp; inv Heqs.
-            break_match_hyp; inv H0.
-            symmetry; eapply handle_gep_addr_preserves_provenance; eauto.
+                destruct l as [_ | h ls].
+                * cbn in MAP.
+                  inv MAP.
+                * exists h.
+                  cbn in MAP.
+                  break_match_hyp; inv MAP.
+                  break_match_hyp; inv H0.
+                  split; cbn; auto.
+
+              + cbn in NTH.
+                destruct l as [_ | h ls].
+                * cbn in MAP.
+                  inv MAP.
+                * cbn in MAP.
+                  break_match_hyp; [break_match_hyp|]; inv MAP.
+                  epose proof (IHres _ _ NTH ls Heqo0) as [y [HF INy]].
+                  exists y; split; cbn; eauto.
+          Qed.
+
+          Lemma Nth_exists :
+            forall {X} (xs : list X) n,
+              n < length xs ->
+              exists x, Nth xs n x.
+          Proof.
+            intros X xs.
+            induction xs; intros n LEN.
+            - cbn in *; lia.
+            - cbn in LEN.
+              destruct n.
+              + exists a; cbn; auto.
+              + cbn.
+                apply IHxs.
+                lia.
+          Qed.
+
+          (* Exists n in ptrs *)
+          pose proof sequence_OOM_length _ _ Heqo as PTRS_LENGTH.
+          assert (length (NoOom p' :: ptrs') = length (one :: ixs)) as PTRS_SHIFTED_LENGTH.
+          {
+            symmetry.
+            eapply map_monad_length with (f:=(fun ix : intptr => handle_gep_addr (DTYPE_I 8) p [DVALUE_IPTR ix])).
+            cbn.
+            red.
+            rewrite Heqs0.
+            rewrite Heqs1.
+            reflexivity.
           }
 
-          rewrite PROV.
-
-          rewrite Heqs0.
-          rewrite IP.from_Z_to_Z with (z:=1%Z) (i:=one); auto.
-
-          assert ((ptr_to_int ptr + Z.of_N (sizeof_dtyp (DTYPE_I 8)) * 1 +
-                     Z.of_N (sizeof_dtyp (DTYPE_I 8)) * IP.to_Z b) =
-                    (ptr_to_int ptr + Z.of_N (sizeof_dtyp (DTYPE_I 8)) * IP.to_Z a))%Z as EQ.
-          { rewrite sizeof_dtyp_i8.
-            unfold Z.of_N.
-
-            rewrite IP.from_Z_to_Z with (z:=(1 + Z.of_nat n)%Z) (i:=a); auto.
-            rewrite IP.from_Z_to_Z with (z:=Z.of_nat n) (i:=b); auto.
+          pose proof intptr_seq_len _ _ _ SEQ as UNSHIFTED_LENGTH.
+          pose proof intptr_seq_len _ _ _ SEQ_SHIFT as SHIFTED_LENGTH.
+          assert (n < S len) as BOUND_n.
+          { apply Nth_ix_lt_length in NTH.
             lia.
           }
 
-          rewrite EQ.
+          pose proof Nth_exists ptrs n as PTRS_n.
+          forward PTRS_n; [lia|].
+          destruct PTRS_n as [ptr_a PTRS_n].
+          
+          (* GEP with a *)
+          apply handle_gep_addr_ix in Heqs0.
+          pose proof Heqs as MAPM.
+          eapply map_monad_err_Nth with (n:=n) in Heqs as [a' [GEP_a' NTH_a']].
+          2: {
+            (* Nth l'' n b *)
+            (* Nth (one :: ixs) n a *)
+            unfold sequence in Heqo.
+
+            eapply map_monad_OOM_Nth with (n:=n) in Heqo as [pa [EQPA NTH_pa]].
+            unfold id in EQPA. inv EQPA.
+            eapply NTH_pa.
+            eapply PTRS_n.
+          }
+
+          cbn in NTH, NTH_a'.
+          rewrite NTH in NTH_a'.
+          inv NTH_a'.
+
+          rewrite sizeof_dtyp_i8 in Heqs0.
+          rewrite from_Z_to_Z with (z:=1%Z) in Heqs0; auto.
+          replace (ptr_to_int p + Z.of_N 1 * 1)%Z
+            with (ptr_to_int p + 1)%Z in Heqs0 by lia.
+
+          (* GEP with b *)
+          assert (handle_gep_addr (DTYPE_I 8) p' [DVALUE_IPTR b] = ret (NoOom ptr_a)) as GEP_b.
+          { rewrite handle_gep_addr_ix' with (p':= ptr_a).
+            reflexivity.
+            pose proof GEP_a' as GEP_a''.
+            apply handle_gep_addr_ix in GEP_a'.
+            rewrite Heqs0.
+            rewrite from_Z_to_Z with (z:=Z.of_nat n); auto.
+            rewrite from_Z_to_Z with (z:=(1 + Z.of_nat n)%Z) in GEP_a'; auto.
+            rewrite sizeof_dtyp_i8.
+            rewrite sizeof_dtyp_i8 in GEP_a'.
+            replace (ptr_to_int p + 1 + Z.of_N 1 * Z.of_nat n)%Z
+              with (ptr_to_int ptr_a) by lia.
+
+            symmetry.
+            eapply int_to_ptr_ptr_to_int.
+
+            (* p' and ptr_a both have the same provenance as p *)
+            assert (address_provenance p' = address_provenance p) as PROV.
+            { rewrite map_monad_unfold in MAPM.
+              cbn in MAPM.
+              break_match_hyp; inv MAPM.
+              break_match_hyp; inv H0.
+              symmetry; eapply handle_gep_addr_preserves_provenance; eauto.
+            }
+
+            assert (address_provenance ptr_a = address_provenance p) as PROV_a.
+            {
+              symmetry; eapply handle_gep_addr_preserves_provenance; eauto.
+            }
+
+            congruence.
+          }
+
+          rewrite GEP_a'.
+          rewrite GEP_b.
           reflexivity.
         }
 
         rewrite Heqs'.
         cbn.
 
+        setoid_rewrite bind_ret_l.
+        rewrite Heqo.
+        cbn.
+
         eapply within_ret_refl; eauto.
+      }
+      { cbn in CONSEC.
+        apply rw_ret_nin_raise in CONSEC; eauto.
+        contradiction.
+      }
   Qed.
 
   Lemma get_consecutive_ptrs_ge :
@@ -1077,8 +1267,7 @@ Module MemoryHelpers (LP : LLVMParams) (MP : MemoryParams LP) (Byte : ByteModule
           2: {
             cbn in CONSEC'.
             setoid_rewrite rbm_raise_bind in CONSEC'; eauto.
-            convert_to_ret_hyp;
-              eapply rw_ret_nin_raise in CONSEC'; eauto; contradiction.
+            eapply rw_ret_nin_raise in CONSEC'; eauto; contradiction.
           }
 
           cbn in CONSEC'.
@@ -1091,23 +1280,47 @@ Module MemoryHelpers (LP : LLVMParams) (MP : MemoryParams LP) (Byte : ByteModule
           break_match_hyp; inv Heqo.
           cbn in CONSEC'.
           break_match_hyp; cbn in CONSEC'.
-          convert_to_ret_hyp;
-            eapply rw_ret_nin_raise in CONSEC'; eauto; contradiction.
+          setoid_rewrite rbm_raise_bind in CONSEC'; eauto.
+          eapply rw_ret_nin_raise in CONSEC'; eauto; contradiction.
           break_match_hyp; cbn in CONSEC'.
-          convert_to_ret_hyp;
-            eapply rw_ret_nin_raise in CONSEC'; eauto; contradiction.
+          setoid_rewrite rbm_raise_bind in CONSEC'; eauto.
+          eapply rw_ret_nin_raise in CONSEC'; eauto; contradiction.
           break_match_hyp; cbn in CONSEC'.
           inv Heqs0.
           break_match_hyp; inv Heqs0.
 
+          setoid_rewrite bind_ret_l in CONSEC'.
+
+          destruct o as [p' | oom_msg].
+          2: {
+            cbn in CONSEC'.
+            eapply rw_ret_nin_raise in CONSEC'; eauto; contradiction.
+          }
+
+          destruct o0 as [p'' | oom_msg].
+          2: {
+            cbn in CONSEC'.
+            eapply rw_ret_nin_raise in CONSEC'; eauto; contradiction.
+          }
+
           apply handle_gep_addr_ix in Heqs.
           apply handle_gep_addr_ix in Heqs1.
-          convert_to_ret_hyp.
+
+          cbn in CONSEC'.
+          break_match_hyp.
+          2: {
+            cbn in CONSEC'.
+            eapply rw_ret_nin_raise in CONSEC'; eauto; contradiction.
+          }
+
+          cbn in CONSEC'.
+
           apply within_ret_ret in CONSEC'; eauto.
           inv CONSEC'.
 
           rewrite sizeof_dtyp_i8 in *.
           erewrite IP.from_Z_to_Z in Heqs1; eauto.
+          break_match_hyp; inv Heqo.
           lia.
         }
         lia.
@@ -1224,12 +1437,19 @@ Module MemoryHelpers (LP : LLVMParams) (MP : MemoryParams LP) (Byte : ByteModule
           destruct (map_monad (fun ix : IP.intptr => handle_gep_addr (DTYPE_I 8) ptr [DVALUE_IPTR ix])
                               (i :: l)) eqn:HMAPM.
           { cbn in CONSEC'.
-            convert_to_ret_hyp.
+            setoid_rewrite rbm_raise_bind in CONSEC'; [|typeclasses eauto].
             eapply rw_ret_nin_raise in CONSEC'; [contradiction | typeclasses eauto].
           }
 
           cbn in CONSEC'.
-          convert_to_ret_hyp.
+          setoid_rewrite bind_ret_l in CONSEC'.
+          destruct (sequence l0) eqn:HSEQUENCE.
+          2: {
+            cbn in CONSEC'.
+            eapply rw_ret_nin_raise in CONSEC'; [contradiction | typeclasses eauto].
+          }
+
+          cbn in CONSEC'.
           apply within_ret_ret in CONSEC'; eauto.
           inv CONSEC'.
           break_match_hyp; inv Heqo0.
@@ -1241,9 +1461,22 @@ Module MemoryHelpers (LP : LLVMParams) (MP : MemoryParams LP) (Byte : ByteModule
           break_match_hyp; inv Heqs0.
           inv HMAPM.
 
+          destruct o as [p' | oom_msg].
+          2: {
+            cbn in HSEQUENCE; inv HSEQUENCE.
+          }
+
+          destruct o0 as [p'' | oom_msg].
+          2: {
+            cbn in HSEQUENCE; inv HSEQUENCE.
+          }
+
           apply handle_gep_addr_ix in Heqs1.
           rewrite sizeof_dtyp_i8 in Heqs1.
           rewrite (IP.from_Z_to_Z _ _ Heqo1) in Heqs1.
+          cbn in HSEQUENCE.
+          break_match_hyp; inv HSEQUENCE.
+          break_match_hyp; inv Heqo2.
           lia.
         }
         lia.
@@ -1300,7 +1533,7 @@ Module MemoryHelpers (LP : LLVMParams) (MP : MemoryParams LP) (Byte : ByteModule
           Util.Nth ptrs ix_nat p ->
           exists ix,
             NoOom ix = IP.from_Z (Z.of_nat ix_nat) /\
-              handle_gep_addr (DTYPE_I 8) ptr [Events.DV.DVALUE_IPTR ix] = inr p).
+              handle_gep_addr (DTYPE_I 8) ptr [Events.DV.DVALUE_IPTR ix] = inr (ret p)).
   Proof.
     intros M HM EQM EQV Pre Post B MB WM WRET OOM ERR LAWS RAISE_OOM RAISE_ERR RWOOM RWERR
       ptr len ptrs CONSEC p ix_nat NTH.
@@ -1320,12 +1553,18 @@ Module MemoryHelpers (LP : LLVMParams) (MP : MemoryParams LP) (Byte : ByteModule
     destruct (map_monad
                 (fun ix : IP.intptr => handle_gep_addr (DTYPE_I 8) ptr [Events.DV.DVALUE_IPTR ix]) l) eqn:MAP.
     { cbn in CONSEC.
-      convert_to_ret_hyp.
+      setoid_rewrite rbm_raise_bind in CONSEC; auto.
       apply rw_ret_nin_raise in CONSEC; try contradiction; auto.
     }
 
     cbn in CONSEC.
-    convert_to_ret_hyp.
+    setoid_rewrite bind_ret_l in CONSEC.
+    destruct (sequence l0) eqn:HSEQUENCE.
+    2: {
+      cbn in CONSEC.
+      apply rw_ret_nin_raise in CONSEC; try contradiction; auto.
+    }
+
     apply within_ret_ret in CONSEC; auto.
     inv CONSEC.
 
@@ -1333,6 +1572,11 @@ Module MemoryHelpers (LP : LLVMParams) (MP : MemoryParams LP) (Byte : ByteModule
     eapply map_monad_err_forall2 in PTRS.
     eapply Forall2_forall in PTRS.
     destruct PTRS as [PTRSLEN PTRS].
+
+    pose proof HSEQUENCE.
+    eapply map_monad_OOM_Nth in HSEQUENCE; eauto.
+    destruct HSEQUENCE as [y [EQY NTHY]].
+    unfold id in EQY; inv EQY.
 
     eapply map_monad_err_Nth in MAP as [ix [P NTH']]; eauto.
     exists ix; split; eauto.
@@ -1355,7 +1599,7 @@ Module MemoryHelpers (LP : LLVMParams) (MP : MemoryParams LP) (Byte : ByteModule
           Util.Nth ptrs ix_nat p ->
           exists ix,
             NoOom ix = IP.from_Z (Z.of_nat ix_nat) /\
-              handle_gep_addr (DTYPE_I 8) ptr [Events.DV.DVALUE_IPTR ix] = inr p).
+              handle_gep_addr (DTYPE_I 8) ptr [Events.DV.DVALUE_IPTR ix] = inr (ret p)).
   Proof.
     intros M HM EQM EQV EQRET B MB OOM ERR LAWS RAISE_OOM RAISE_ERR
       ptr len ptrs CONSEC p ix_nat NTH.
@@ -1439,22 +1683,44 @@ Module MemoryHelpers (LP : LLVMParams) (MP : MemoryParams LP) (Byte : ByteModule
     intros M HM OOM ERR EQM' EQV LAWS RAISE ptr len.
     unfold get_consecutive_ptrs.
     destruct (intptr_seq 0 len) eqn:HSEQ.
-    - right.
-
-      pose proof (map_monad_err_succeeds
+    - pose proof (map_monad_err_succeeds
                     (fun ix : IP.intptr => handle_gep_addr (DTYPE_I 8) ptr [Events.DV.DVALUE_IPTR ix]) l) as HMAPM.
       forward HMAPM.
       { intros a IN.
-        eexists; eapply handle_gep_addr_ix'.
-        reflexivity.
+        destruct (int_to_ptr (ptr_to_int ptr + Z.of_N (sizeof_dtyp (DTYPE_I 8)) * IP.to_Z a)%Z (address_provenance ptr)) eqn:IX.
+        - exists (ret a0).
+          apply handle_gep_addr_ix'; cbn; auto.
+        - eapply handle_gep_addr_ix'_OOM in IX; auto.
+          destruct IX as [msg IX].
+          exists (Oom msg).
+          cbn; auto.
       }
 
       destruct HMAPM as (ptrs & HMAPM).
-      exists ptrs.
-      cbn.
-      rewrite bind_ret_l.
-      rewrite HMAPM.
-      reflexivity.
+
+      destruct (sequence ptrs) eqn:HSEQUENCE.
+      { rename l0 into ptrs'.
+        right.
+        exists ptrs'.
+        cbn.
+        rewrite bind_ret_l.
+        rewrite HMAPM.
+        setoid_rewrite bind_ret_l.
+        rewrite HSEQUENCE.
+        cbn.
+        reflexivity.
+      }
+
+      { left.
+        exists s.
+        cbn.
+        rewrite bind_ret_l.
+        rewrite HMAPM.
+        setoid_rewrite bind_ret_l.
+        rewrite HSEQUENCE.
+        cbn.
+        reflexivity.
+      }
     - left.
       exists s.
       cbn.
@@ -1501,15 +1767,26 @@ Module MemoryHelpers (LP : LLVMParams) (MP : MemoryParams LP) (Byte : ByteModule
                   (fun ix : IP.intptr => handle_gep_addr (DTYPE_I 8) ptr [Events.DV.DVALUE_IPTR ix]) l) as HMAPM.
       forward HMAPM.
       { intros a IN.
-        eexists; eapply handle_gep_addr_ix'.
-        reflexivity.
+        destruct (int_to_ptr (ptr_to_int ptr + Z.of_N (sizeof_dtyp (DTYPE_I 8)) * IP.to_Z a)%Z (address_provenance ptr)) eqn:IX.
+        - exists (ret a0).
+          apply handle_gep_addr_ix'; cbn; auto.
+        - eapply handle_gep_addr_ix'_OOM in IX; auto.
+          destruct IX as [msg' IX].
+          exists (Oom msg').
+          cbn; auto.
       }
 
       destruct HMAPM as (ptrs & HMAPM).
       rewrite HMAPM in CONTRA.
       cbn in CONTRA.
 
-      convert_to_raise_hyp.
+      setoid_rewrite bind_ret_l in CONTRA.
+      destruct (sequence ptrs) eqn:HSEQUENCE.
+      2: {
+        cbn in CONTRA.
+        eapply disjoint_raise_within in CONTRA; eauto.
+      }
+
       eapply rw_raise_nin_ret in CONTRA; eauto.
   Qed.
 
@@ -3931,7 +4208,11 @@ Module Type MemoryExecMonad (LP : LLVMParams) (MP : MemoryParams LP) (MMSP : Mem
     apply exec_correct_lift_OOM.
 
     intros * RUN.
+    eapply exec_correct_bind.
     apply exec_correct_lift_err_RAISE_ERROR.
+
+    intros a0 ms_init0 ms_after_m0 st_init0 st_after_m0 H.
+    apply exec_correct_lift_OOM.
   Qed.
 
   Lemma exec_correct_fresh_sid :
@@ -5332,17 +5613,63 @@ Module MemStateInfiniteHelpers (LP : LLVMParamsBig) (MP : MemoryParams LP) (MMSP
 
     forward HMAPM.
     { intros a IN.
-      eexists.
-      eapply handle_gep_addr_ix'.
-      reflexivity.
+      destruct (int_to_ptr (ptr_to_int ptr + Z.of_N (sizeof_dtyp (DTYPE_I 8)) * LP.IP.to_Z a)%Z (address_provenance ptr)) eqn:IX.
+      - exists (ret a0).
+        apply handle_gep_addr_ix'; cbn; auto.
+      - eapply handle_gep_addr_ix'_OOM in IX; auto.
+        destruct IX as [msg' IX].
+        exists (Oom msg').
+        cbn; auto.
     }
 
     destruct HMAPM as (res & HMAPM).
-    exists res.
-    rewrite bind_ret_l.
-    rewrite HMAPM.
-    cbn.
-    reflexivity.
+    destruct (Monads.sequence res) eqn:HSEQUENCE.
+    { rename l into ptrs.
+      exists ptrs.
+      rewrite bind_ret_l.
+      rewrite HMAPM.
+      cbn.
+      rewrite bind_ret_l.
+      rewrite HSEQUENCE.
+      cbn.
+      reflexivity.
+    }
+    { (* TODO: move this *)
+      Set Nested Proofs Allowed.
+      (* TODO: can I generalize this? *)
+      Lemma map_monad_OOM_fail :
+        forall {A B} (f : A -> OOM B) l b,
+          map_monad f l = Oom b ->
+          exists a, In a l /\ f a = Oom b.
+      Proof.
+        intros A B f l b MAP.
+        generalize dependent b.
+        generalize dependent l.
+        induction l; intros b MAP.
+        - cbn in MAP.
+          inv MAP.
+        - cbn.
+          cbn in MAP.
+          destruct (f a) eqn:Hfa; inv MAP.
+          + rename H0 into MAP.
+            destruct (map_monad f l) eqn:HMAP; inv MAP.
+            specialize (IHl b eq_refl) as [a' [IN FA]].
+            exists a'. tauto.
+          + exists a. split; auto.
+      Qed.
+
+      apply map_monad_OOM_fail in HSEQUENCE as [a [IN EQA]].
+      unfold id in EQA. subst.
+
+      pose proof map_monad_err_In _ _ _ _ HMAPM IN as [ix [GEP INix]].
+      apply handle_gep_addr_ix_OOM in GEP; auto.
+      destruct GEP as [msg' GEP].
+      pose proof
+        (LP.I2P_BIG.int_to_ptr_safe (ptr_to_int ptr + Z.of_N (sizeof_dtyp (DTYPE_I 8)) * to_Z ix)
+           (address_provenance ptr)) as SAFE.
+      rewrite GEP in SAFE.
+      contradiction.
+    }
   Qed.
 
 End MemStateInfiniteHelpers.
